Add R2rHP <-> R2rHC proof in Coq, and link in the TR

Criteria2.v
@@ -149,6 +149,7 @@ Qed.
 Lemma rewriting_lemma : forall t1 t2,
     (forall m, prefix m t1 -> prefix m t2) ->
     (forall π, π t1 -> π t2).
+Proof.
 Admitted.
 
 Theorem RobsP_RPP : (forall P π, Observable π -> RP P π) <->
@@ -468,14 +469,51 @@ Proof.
     { clear. intros Cs m1 m2 Hsem1 Hsem2. exists Cs; now auto. }
     specialize (H H' Ct m1 m2 Hsem1 Hsem2). now assumption.
 Qed.
+(*************************************************************************)
+(* Robust 2-relational Hyperproperty Preservation *)
+(*************************************************************************)
 
+Definition r2HRP : Prop :=
+  forall P1 P2 r, (hrsat2 P1 P2 r) -> (hrsat2 (P1 ↓) (P2 ↓) r).
+
+Definition r2HRC : Prop :=
+  forall P1 P2 Ct, exists Cs, (sem src (Cs [P1]) = sem tgt (Ct [P1 ↓]))
+                    /\ (sem src (Cs [P2]) = sem tgt (Ct [P2 ↓])).
+
+
+Theorem r2HRP_r2HRC : r2HRP <-> r2HRC.
+Proof.
+  unfold r2HRP, r2HRC; split.
+  - intros H2hrp P1 P2 Ct. apply NNPP. intros ff.
+    rewrite not_ex_forall_not in ff.
+    specialize (H2hrp P1 P2).
+    specialize (H2hrp (fun f1 f2 => exists Cs, forall t, f1 t = sem src (Cs [ P1 ]) t
+                                                   /\ f2 t = sem src (Cs [ P2 ]) t)).
+    simpl in *.
+    assert (hh : hrsat2 P1 P2
+            (fun f1 f2 : prop =>
+             exists Cs : ctx src,
+               forall t : trace, f1 t = sem src (Cs [P1]) t /\ f2 t = sem src (Cs [P2]) t)).
+    { clear. unfold hrsat2. intros. exists C. intros. split; now auto. }
+    specialize (H2hrp hh Ct); clear hh.
+    unfold hrsat2 in H2hrp. destruct H2hrp as [Cs h].
+    specialize (ff Cs). 
+    assert (sem src (Cs [P1]) = sem tgt (Ct [P1 ↓])).
+    { apply functional_extensionality. intros t. specialize (h t).
+      destruct h as [h1 h2]. auto. }
+    assert (sem src (Cs [P2]) = sem tgt (Ct [P2 ↓])).
+    { apply functional_extensionality. intros t. specialize (h t).
+      destruct h as [h1 h2]. auto. }
+    apply ff. split; auto.
+  - intros h P1 P2 r hcs Ct. destruct (h P1 P2 Ct) as [Cs [h0 h1]]; clear h.
+    specialize (hcs Cs).
+    rewrite h0, h1 in hcs. now assumption.
+Qed.
 
 (*************************************************************************)
 (* Robust 2-rel HyperProperty Pres => trace equivalence pres             *)
 (*************************************************************************)
 
-Definition r2HRP : Prop :=
-  forall P1 P2 r, (hrsat2 P1 P2 r) -> (hrsat2 (P1 ↓) (P2 ↓) r).
 
 Lemma r2HRP_teq : r2HRP -> teq_preservation.
 Proof.
@@ -496,7 +534,7 @@ Section source_determinism.
 
   Hypothesis src_det : forall P t1 t2, sem src P t1 -> sem src P t2 -> t1 = t2.
 
-  Theorem two_RC_teq_preservation : r2RC -> teq_preservation.
+  Theorem two_RSC_teq_preservation : r2RC -> teq_preservation.
   Proof.
     unfold r2RC. rewrite teq'. intros H P1 P2 [Ct [t' H']].   
     rewrite not_iff in H'. destruct H' as [[H1' nH2'] | [nH1' H2']].
@@ -508,12 +546,7 @@ Section source_determinism.
       destruct (H _ _ _ _ _ H1' H2') as [Cs [H1 H2]].
       exists Cs, t'. intros Hf. rewrite <- Hf in H2. 
       specialize (src_det (Cs [P1] ) t1 t' H1 H2). now subst.
-  Qed.
-
-  Theorem r2RPP_teq_preservation : r2RPP -> teq_preservation.
-  Proof.
-    rewrite r2RPP_r2RC. now apply two_RC_teq_preservation.
-  Qed. 
+   Qed.
   
 End source_determinism.
 
